execution/theories/SerializableDerive.v
@@ -1,0 +1,553 @@
+From ConCert.Execution Require Import Serializable.
+From ConCert.Execution Require Import Monad.
+From ConCert.Execution Require Import OptionMonad.
+From Coq Require Import List.
+
+Import ListNotations.
+
+
+Inductive Bool :=
+| _true : bool -> nat -> Bool
+| _false : bool -> Bool.
+
+Module oldLtac.
+  Ltac make_serializer_case ty :=
+    match ty with
+    | ?T1 -> ?T2 =>
+      let rest := make_serializer_case T2 in
+      constr:(fun (f : SerializedValue -> SerializedValue) (v : T1) =>
+                rest (fun (cur : SerializedValue) => f (serialize (v, cur))))
+    | SerializedValue =>
+      constr:(fun (f : SerializedValue -> SerializedValue) => f (serialize tt))
+    end.
+
+  Ltac make_serializer_aux term tag :=
+    match type of term with
+    | ?T1 -> (?T2 -> ?T3) =>
+      let cs := make_serializer_case T1 in
+      let cs := constr:(cs (fun x => serialize (tag, x))) in
+      let term := (eval hnf in (term cs)) in
+      make_serializer_aux term (S tag)
+    | ?T -> SerializedValue =>
+      term
+    end.
+
+  Ltac make_serializer eliminator :=
+    let term := (eval hnf in (eliminator (fun _ => SerializedValue))) in
+    let serializer := make_serializer_aux term 0 in
+    eval cbn in serializer.
+
+  Ltac make_deserializer_case ty :=
+    match ty with
+    | ?T1 -> ?T2 =>
+      let rest := make_deserializer_case T2 in
+      constr:(fun builder sv =>
+                do '(a, sv) <- (deserialize sv : option (T1 * SerializedValue));
+                rest (builder a) sv)
+    | ?T => constr:(fun (value : T) (sv : SerializedValue) =>
+                do _ <- (deserialize sv : option unit);
+                Some value)
+    end.
+
+  Ltac make_deserializer_aux ctors rty :=
+    match ctors with
+    | (?ctor, ?tl) =>
+      let ty := type of ctor in
+      let cs := make_deserializer_case ty in
+      let rest := make_deserializer_aux tl rty in
+      constr:(
+        fun tag sv =>
+          match tag with
+          | 0 => cs ctor sv
+          | S tag => rest tag sv
+          end)
+    | tt => constr:(fun (tag : nat) (sv : SerializedValue) => @None rty)
+    end.
+
+  Ltac make_deserializer ctors rty :=
+    let deser := make_deserializer_aux ctors rty in
+    let deser := constr:(fun sv => do '(tag, sv) <- deserialize sv; deser tag sv) in
+    deser.
+      (* eval cbn in deser. *)
+
+  Ltac get_ty_from_elim_ty ty :=
+    match ty with
+    | forall (_ : ?T -> Type), _ => T
+    end.
+
+  Ltac make_serializable eliminator ctors :=
+    let ser := make_serializer eliminator in
+    let elim_ty := type of eliminator in
+    let ty := get_ty_from_elim_ty elim_ty in
+    let deser := make_deserializer ctors ty in
+    exact
+      {| serialize := ser;
+        deserialize := deser;
+        deserialize_serialize :=
+          ltac:(intros []; repeat (cbn in *; try rewrite deserialize_serialize; auto)) |}.
+
+  Notation "'Derive' 'Serializable' rect" :=
+    ltac:(make_serializable rect tt) (at level 0, rect at level 10, only parsing).
+
+  Notation "'Derive' 'Serializable' rect < c0 , .. , cn >" :=
+    (let pairs := pair c0 .. (pair cn tt) .. in
+    ltac:(
+      (* This matches last-to-first so it always finds 'pairs' *)
+      match goal with
+      | [pairs := ?x |- _] => make_serializable rect x
+      end))
+      (at level 0, rect at level 10, c0, cn at level 9, only parsing).
+
+    #[local]
+  Instance test : Serializable Bool := Derive Serializable Bool_rect < _true, _false >.
+  (* Print test. *)
+  (* MetaCoq Run (tmQuote (Derive Serializable Bool_rect < _true, _false >) >>= tmPrint). *)
+End oldLtac.
+
+Module newLtac.
+  (* Check Bool_rect. *)
+  (* Eval hnf in (Bool_rect (fun _ => SerializedValue)). *)
+
+  Require Import Ltac2.Ltac2.
+
+  Local Ltac2 rec get_constructors_fix (data : Ind.data) (n : int) : constructor list :=
+    match Int.equal n 0 with
+    | true => []
+    | false =>
+      let n' := Int.sub n 1 in
+      (Ind.get_constructor data n') :: (get_constructors_fix data n')
+    end.
+
+  Local Ltac2 get_constructors (ty : constr) : constructor list :=
+    match Constr.Unsafe.kind ty with
+    | Constr.Unsafe.Ind ind _ =>
+      let data := Ind.data ind in
+      let n := Ind.nconstructors data in
+      get_constructors_fix data n
+    | _ => Control.throw (Invalid_argument
+      (Some (Message.of_string "Not an inductive type")))
+    end.
+
+  Local Ltac2 make_serializer_aux a b : constr :=
+    let a_ty := Constr.type a in
+    a.
+  (*
+  Ltac make_serializer_aux term tag :=
+    match type of term with
+    | ?T1 -> (?T2 -> ?T3) =>
+      let cs := make_serializer_case T1 in
+      let cs := constr:(cs (fun x => serialize (tag, x))) in
+      let term := (eval hnf in (term cs)) in
+      make_serializer_aux term (S tag)
+    | ?T -> SerializedValue =>
+      term
+    end.
+
+  *)
+
+  Local Ltac2 make_serializer rect : constr :=
+    let term := Std.eval_hnf (rect (fun _ => constr:(SerializedValue))) in
+    let serializer := make_serializer_aux term 0 in
+    Std.eval_cbn {
+      Std.rBeta := false;
+      Std.rMatch := false;
+      Std.rFix := false;
+      Std.rCofix := false;
+      Std.rZeta := false;
+      Std.rDelta := false;
+      Std.rConst := [] } serializer.
+
+(*   Ltac2 derive_serializable (ty : constr) (rect : constr) :=
+    let ctors := get_constructors ty in
+    let ser := make_serializer rect in
+    (* let deser := make_deserializer ctors ty in *)
+    exact (True). *)
+  (* exact
+      {| serialize := ser;
+        deserialize := deser;
+        deserialize_serialize :=
+          ltac:(intros []; repeat (cbn in *; try rewrite deserialize_serialize; auto)) |}. *)
+
+  (*
+
+  Ltac make_serializer_case ty :=
+    match ty with
+    | ?T1 -> ?T2 =>
+      let rest := make_serializer_case T2 in
+      constr:(fun (f : SerializedValue -> SerializedValue) (v : T1) =>
+                rest (fun (cur : SerializedValue) => f (serialize (v, cur))))
+    | SerializedValue =>
+      constr:(fun (f : SerializedValue -> SerializedValue) => f (serialize tt))
+    end.
+
+  Ltac make_serializer_aux term tag :=
+    match type of term with
+    | ?T1 -> (?T2 -> ?T3) =>
+      let cs := make_serializer_case T1 in
+      let cs := constr:(cs (fun x => serialize (tag, x))) in
+      let term := (eval hnf in (term cs)) in
+      make_serializer_aux term (S tag)
+    | ?T -> SerializedValue =>
+      term
+    end.
+  *)
+(*   Compute (
+    let x := ltac2:(derive_serializable constr:(Bool) constr:(Bool_rect)) in x).
+  Compute (
+    let x := ltac2:(derive_serializable constr:(0)) in x). *)
+End newLtac.
+
+
+
+From MetaCoq.Template Require Import Ast.
+From MetaCoq.Template Require Import AstUtils.
+From MetaCoq.Template Require Import BasicAst.
+From MetaCoq.Template Require Import Loader.
+From MetaCoq.Template Require Import TemplateMonad.
+From MetaCoq.Template Require Import monad_utils.
+From MetaCoq.Template Require Import utils.
+
+Import MCMonadNotation.
+
+Global Unset Asymmetric Patterns.
+Local Set Universe Polymorphism.
+
+Definition get_inductive (T : Type) : TemplateMonad inductive := 
+  Tast <- tmQuote T;;
+  match Tast with
+  | tInd ind _ => ret ind
+  | tApp (tInd ind _) _ => ret ind
+  | _ => tmFail "Cannot extract inductive, are you sure you passed a type?"
+  end.
+
+  Definition get_inductive_ (t : term) : TemplateMonad inductive := 
+  match t with
+  | tInd ind _ => ret ind
+  | tApp (tInd ind _) _ => ret ind
+  | _ => tmFail "Cannot extract inductive, are you sure you passed a type?"
+  end.
+
+Definition get_mib (ind : inductive) : TemplateMonad mutual_inductive_body :=
+  tmQuoteInductive (inductive_mind ind).
+
+Definition get_nth_oib (mib : mutual_inductive_body) (n : nat) : TemplateMonad one_inductive_body :=
+  match nth_error (ind_bodies mib) n with
+  | Some oib => ret oib
+  | None => tmFail "Could not find inductive in mutual inductive?"
+  end.
+
+Definition get_oib (mib : mutual_inductive_body) (ind : inductive) : TemplateMonad one_inductive_body :=
+  get_nth_oib mib (inductive_ind ind).
+
+Definition get_constructors (oib : one_inductive_body) : list constructor_body :=
+  ind_ctors oib.
+
+Definition instance_exists (T : Type) : TemplateMonad unit :=
+  inst <- tmInferInstance None T;;
+  match inst with
+  | my_Some _ _ => ret tt
+  | _ => tmFail "Instance already exist"
+  end.
+
+Definition qualid_const_kername (q : qualid) : TemplateMonad kername :=
+  glob_ref <- tmLocate1 q;;
+  match glob_ref with
+  | ConstRef kn => ret kn
+  | _ => tmFail "Unexpected global_reference after unquoting"
+  end.
+
+Definition register_instance (q : qualid) : TemplateMonad unit :=
+  tmLocate1 q >>= tmExistingInstance.
+
+Definition get_rect (oib : one_inductive_body) : TemplateMonad kername :=
+  let name := (ind_name oib) ^ "_rect" in
+  qualid_const_kername name.
+
+
+
+Definition make_serializer_case : TemplateMonad term :=
+  todo "".
+Definition make_serializer_aux : TemplateMonad term :=
+  todo "".
+Definition make_serializer (eliminator : kername) : TemplateMonad term :=
+  todo "".
+
+Definition deser_case_prod_body :=
+  (fun (T1 T2 T : Type)
+       (rest : (T2 -> T) -> SerializedValue -> option T)
+       (serT1 : Serializable T1) =>
+  (fun builder sv =>
+              do '(a, sv) <- (@deserialize (T1 * SerializedValue) _ sv);
+              rest (builder a) sv)).
+Definition deser_case_ind_body :=
+  (fun (T : Type) =>
+  (fun (value : T) (sv : SerializedValue) =>
+                match @deserialize unit _ sv with
+                | Some _ => Some value
+                | None => None
+                end)).
+              (* do _ <- (@deserialize unit _ sv); *)
+              (* Some value)). *)
+
+Fixpoint make_deserializer_case (t : term) (T : term) : TemplateMonad term :=
+  match t with
+  | tProd _ T1 T2 =>
+      rest <- make_deserializer_case T2 T;;
+      ret (tApp
+        <% @deser_case_prod_body %>
+        [T1; T2; T; rest; hole])
+  | tRel _ =>
+      ret (tApp
+        <% @deser_case_ind_body %>
+        [t]
+      )
+  | _ => 
+      tmFail "err 1"
+  end.
+
+Definition deser_aux_cons_body :=
+  (fun (T ctorT : Type)
+       (cs : ctorT -> SerializedValue -> option T)
+       (rest : nat -> SerializedValue -> option T)
+       (ctor : ctorT) =>
+  (fun (tag : nat) (sv : SerializedValue) =>
+        match tag with
+        | 0 => cs ctor sv
+        | S tag => rest tag sv
+        end)).
+Definition deser_aux_nil_body :=
+  (fun (T : Type) =>
+  (fun (tag : nat) (sv : SerializedValue) => @None T)).
+
+Fixpoint make_deserializer_aux (ctors : list constructor_body) (T : term) (i : nat) : TemplateMonad term :=
+  match ctors with
+  | ctor :: tl =>
+    let ty := ctor.(cstr_type) in
+    ind <- get_inductive_ T;;
+    let ctor := (tConstruct ind i []) in
+    cs <- make_deserializer_case ty T;;
+    rest <- make_deserializer_aux tl T (S i);;
+    ret (
+      tApp
+        <% deser_aux_cons_body %>
+        [T; ty; cs; rest; ctor]
+    )
+  | [] =>
+    ret (tApp <% deser_aux_nil_body %> [T])
+  end.
+
+Definition deser_body :=
+  (fun (T : Type) =>
+    (fun (deser : nat -> SerializedValue -> option T) =>
+      (fun sv =>
+        do '(tag, sv) <- @deserialize (nat * SerializedValue) _ sv;
+        deser tag sv))).
+
+Definition make_deserializer (ctors : list constructor_body) (T : Type) : TemplateMonad term :=
+  tAst <- tmQuote T;;
+  deser <- make_deserializer_aux ctors tAst 0;;
+  let body :=
+    tLambda
+      {| binder_name := nNamed "sv"; binder_relevance := Relevant |}
+      <% SerializedValue %>
+      (tApp
+        <% deser_body %>
+        [tAst; deser; tRel 0]
+      ) in 
+  (* body <- tmEval cbv body;; *)
+  ret deser.
+
+Unset MetaCoq Strict Unquote Universe Mode.
+(* Set MetaCoq Debug. *)
+
+MetaCoq Run (
+  let T := Bool in
+  ind <- get_inductive T;;
+  mib <- get_mib ind;;
+  oib <- get_oib mib ind;;
+  let ctors := get_constructors oib in
+  cs <- match ctors with
+  | h :: h2 :: t =>
+    tAst <- tmQuote T;;
+    let ty := h2.(cstr_type) in
+    match ty with
+    | tProd _ T1 T2 =>
+        rest <- make_deserializer_case T2 tAst;;
+        ret (tApp
+          <% deser_case_prod_body %>
+          [T1; T2; tAst; rest; hole])
+    | tRel _ =>
+        ret (tApp
+          <% @deser_case_ind_body %>
+          [tAst]
+        )
+    | _ => 
+        tmFail "err 1"
+    end
+  | _ => tmFail "t"
+  end;;
+      (* tmPrint cs *)
+    tmMkDefinition "test1" cs
+  ).
+
+
+
+
+
+  let T := Bool in
+  ind <- get_inductive T;;
+  mib <- get_mib ind;;
+  oib <- get_oib mib ind;;
+  let ctors := get_constructors oib in
+  match ctors with
+  | h :: h2 :: t =>
+    tAst <- tmQuote T;;
+    let ty := h2.(cstr_type) in
+    cs <- make_deserializer_case ty tAst;;
+    (* cs <- tmEval cbv cs;; *)
+    (* cs <- tmEval hnf cs;; *)
+    (* tmPrint cs *)
+    tmMkDefinition "test1" cs
+  | _ => tmFail "t"
+  end).
+
+
+MetaCoq Run (
+  let T := Bool in
+  ind <- get_inductive T;;
+  mib <- get_mib ind;;
+  oib <- get_oib mib ind;;
+  let ctors := get_constructors oib in
+  (* tmPrint ctors). *)
+  body <- make_deserializer ctors T;;
+  (* tmPrint body). *)
+  tmMkDefinition "test1" body
+).
+Print test1.
+Eval cbv in test1.
+
+
+Program Definition make_serializable (T : Type) : TemplateMonad unit :=
+  ind <- get_inductive T;;
+  mib <- get_mib ind;;
+  oib <- get_oib mib ind;;
+  eliminator <- get_rect oib;;
+  let ctors := get_constructors oib in
+
+  ser <- make_serializer eliminator;;
+  deser <- make_deserializer ctors T;;
+  (* @ret _ _ _ tt. *)
+  todo "".
+
+
+
+
+Definition make_setters (T : Type) :=
+  Tast <- tmQuote T;;
+  (* ret Tast. *)
+  ind <- match Tast with
+      | tInd ind _ => ret ind
+      | tApp (tInd ind _) _ => ret ind
+      | _ => tmFail "Cannot extract inductive, are you sure you passed a type?"
+      end;;
+  (* ret ind. *)
+  mib <- tmQuoteInductive (inductive_mind ind);;
+  oib <- match nth_error (ind_bodies mib) (inductive_ind ind) with
+         | Some oib => ret oib
+         | None => tmFail "Could not find inductive in mutual inductive?"
+         end;;
+  (* ctors <- ind_ctors oib;; *)
+(*   '(ctor, ar) <- match ind_ctors oib with
+                 | [c] => ret (c.(cstr_type), c.(cstr_arity))
+                 | _ => tmFail "Type should have exactly one constructor"
+                 end;; *)
+  ret (ind_ctors oib).
+
+MetaCoq Run (x <- make_setters Bool;; tmPrint x).
+
+
+Ltac make_serializer_case ty :=
+  match ty with
+  | ?T1 -> ?T2 =>
+    let rest := make_serializer_case T2 in
+    constr:(fun (f : SerializedValue -> SerializedValue) (v : T1) =>
+              rest (fun (cur : SerializedValue) => f (serialize (v, cur))))
+  | SerializedValue =>
+    constr:(fun (f : SerializedValue -> SerializedValue) => f (serialize tt))
+  end.
+
+Ltac make_serializer_aux term tag :=
+  match type of term with
+  | ?T1 -> (?T2 -> ?T3) =>
+    let cs := make_serializer_case T1 in
+    let cs := constr:(cs (fun x => serialize (tag, x))) in
+    let term := (eval hnf in (term cs)) in
+    make_serializer_aux term (S tag)
+  | ?T -> SerializedValue =>
+    term
+  end.
+
+Ltac make_serializer eliminator :=
+  let term := (eval hnf in (eliminator (fun _ => SerializedValue))) in
+  let serializer := make_serializer_aux term 0 in
+  eval cbn in serializer.
+
+Ltac make_deserializer_case ty :=
+  match ty with
+  | ?T1 -> ?T2 =>
+    let rest := make_deserializer_case T2 in
+    constr:(fun builder sv =>
+              do '(a, sv) <- (deserialize sv : option (T1 * SerializedValue));
+              rest (builder a) sv)
+  | ?T => constr:(fun (value : T) (sv : SerializedValue) =>
+              do _ <- (deserialize sv : option unit);
+              Some value)
+  end.
+
+Ltac make_deserializer_aux ctors rty :=
+  match ctors with
+  | (?ctor, ?tl) =>
+    let ty := type of ctor in
+    let cs := make_deserializer_case ty in
+    let rest := make_deserializer_aux tl rty in
+    constr:(
+      fun tag sv =>
+        match tag with
+        | 0 => cs ctor sv
+        | S tag => rest tag sv
+        end)
+  | tt => constr:(fun (tag : nat) (sv : SerializedValue) => @None rty)
+  end.
+
+Ltac make_deserializer ctors rty :=
+  let deser := make_deserializer_aux ctors rty in
+  let deser := constr:(fun sv => do '(tag, sv) <- deserialize sv; deser tag sv) in
+  eval cbn in deser.
+
+Ltac get_ty_from_elim_ty ty :=
+  match ty with
+  | forall (_ : ?T -> Type), _ => T
+  end.
+
+Ltac make_serializable eliminator ctors :=
+  let ser := make_serializer eliminator in
+  let elim_ty := type of eliminator in
+  let ty := get_ty_from_elim_ty elim_ty in
+  let deser := make_deserializer ctors ty in
+  exact
+    {| serialize := ser;
+      deserialize := deser;
+      deserialize_serialize :=
+        ltac:(intros []; repeat (cbn in *; try rewrite deserialize_serialize; auto)) |}.
+
+Notation "'Derive' 'Serializable' rect" :=
+  ltac:(make_serializable rect tt) (at level 0, rect at level 10, only parsing).
+
+Notation "'Derive' 'Serializable' rect < c0 , .. , cn >" :=
+  (let pairs := pair c0 .. (pair cn tt) .. in
+  ltac:(
+    (* This matches last-to-first so it always finds 'pairs' *)
+    match goal with
+    | [pairs := ?x |- _] => make_serializable rect x
+    end))
+    (at level 0, rect at level 10, c0, cn at level 9, only parsing).
