execution/theories/test.v
@@ -1,0 +1,34 @@
+From Equations Require Import Equations.
+
+Class TT (T : Type) := {
+
+}.
+
+Inductive Bool :=
+| bTrue : Bool
+| bFalse : Bool.
+
+
+
+Derive TT for Bool.
+
+
+
+
+
+
+From MetaCoq.Template Require Import Ast.
+From MetaCoq.Template Require Import AstUtils.
+From MetaCoq.Template Require Import BasicAst.
+From MetaCoq.Template Require Import Loader.
+From MetaCoq.Template Require Import TemplateMonad.
+From MetaCoq.Template Require Import monad_utils.
+From MetaCoq.Template Require Import utils.
+
+Import MCMonadNotation.
+
+Global Unset Asymmetric Patterns.
+
+
+
+
